examples/containers/hs-spec/IntSetProperties.v
@@ -71,7 +71,7 @@ Import Test.QuickCheck.Property.Notations.
 
 (* Skipping definition `IntSetProperties.test_split' *)
 
-Definition forValid {a} `{Test.QuickCheck.Property.Testable a}
+#[global] Definition forValid {a} `{Test.QuickCheck.Property.Testable a}
    : (Data.IntSet.Internal.IntSet -> a) -> Prop :=
   fun f =>
     Test.QuickCheck.Property.forAll Test.QuickCheck.Arbitrary.arbitrary (fun t =>
@@ -111,29 +111,30 @@ Definition forValid {a} `{Test.QuickCheck.Property.Testable a}
                                                                                                                 (f
                                                                                                                  t))))).
 
-Definition forValidUnitTree {a} `{Test.QuickCheck.Property.Testable a}
+#[global] Definition forValidUnitTree {a} `{Test.QuickCheck.Property.Testable a}
    : (Data.IntSet.Internal.IntSet -> a) -> Prop :=
   fun f => forValid f.
 
-Definition prop_Valid : Prop :=
+#[global] Definition prop_Valid : Prop :=
   forValidUnitTree (fun t => IntSetValidity.valid t).
 
-Definition prop_EmptyValid : Prop :=
+#[global] Definition prop_EmptyValid : Prop :=
   IntSetValidity.valid Data.IntSet.Internal.empty.
 
-Definition prop_SingletonValid : Coq.Numbers.BinNums.N -> Prop :=
+#[global] Definition prop_SingletonValid : Coq.Numbers.BinNums.N -> Prop :=
   fun x => IntSetValidity.valid (Data.IntSet.Internal.singleton x).
 
-Definition prop_InsertIntoEmptyValid : Coq.Numbers.BinNums.N -> Prop :=
+#[global] Definition prop_InsertIntoEmptyValid
+   : Coq.Numbers.BinNums.N -> Prop :=
   fun x =>
     IntSetValidity.valid (Data.IntSet.Internal.insert x Data.IntSet.Internal.empty).
 
-Definition prop_Single : Coq.Numbers.BinNums.N -> bool :=
+#[global] Definition prop_Single : Coq.Numbers.BinNums.N -> bool :=
   fun x =>
     (Data.IntSet.Internal.insert x Data.IntSet.Internal.empty GHC.Base.==
      Data.IntSet.Internal.singleton x).
 
-Definition prop_Member
+#[global] Definition prop_Member
    : list Coq.Numbers.BinNums.N -> Coq.Numbers.BinNums.N -> bool :=
   fun xs n =>
     let m := Data.IntSet.Internal.fromList xs in
@@ -141,7 +142,7 @@ Definition prop_Member
                          Data.IntSet.Internal.member k m GHC.Base.== (Data.Foldable.elem k xs)) (cons n
                                                                                                       xs).
 
-Definition prop_NotMember
+#[global] Definition prop_NotMember
    : list Coq.Numbers.BinNums.N -> Coq.Numbers.BinNums.N -> bool :=
   fun xs n =>
     let m := Data.IntSet.Internal.fromList xs in
@@ -159,7 +160,7 @@ Definition prop_NotMember
 
 (* Skipping definition `IntSetProperties.prop_LookupGE' *)
 
-Definition prop_InsertDelete
+#[global] Definition prop_InsertDelete
    : Coq.Numbers.BinNums.N -> Data.IntSet.Internal.IntSet -> Prop :=
   fun k t =>
     negb (Data.IntSet.Internal.member k t) Test.QuickCheck.Property.==>
@@ -167,7 +168,7 @@ Definition prop_InsertDelete
      IntSetValidity.valid t' Test.QuickCheck.Property..&&.(**)
      (t' Test.QuickCheck.Property.=== t)).
 
-Definition prop_MemberFromList : list Coq.Numbers.BinNums.N -> bool :=
+#[global] Definition prop_MemberFromList : list Coq.Numbers.BinNums.N -> bool :=
   fun xs =>
     let abs_xs :=
       Coq.Lists.List.flat_map (fun x =>
@@ -179,26 +180,26 @@ Definition prop_MemberFromList : list Coq.Numbers.BinNums.N -> bool :=
                                          Data.IntSet.Internal.notMember arg_3__ t) GHC.Base.∘
                                       GHC.Num.negate) abs_xs).
 
-Definition prop_UnionInsert
+#[global] Definition prop_UnionInsert
    : Coq.Numbers.BinNums.N -> Data.IntSet.Internal.IntSet -> Prop :=
   fun x t =>
     let 't' := Data.IntSet.Internal.union t (Data.IntSet.Internal.singleton x) in
     IntSetValidity.valid t' Test.QuickCheck.Property..&&.(**)
     (t' Test.QuickCheck.Property.=== Data.IntSet.Internal.insert x t).
 
-Definition prop_UnionAssoc
+#[global] Definition prop_UnionAssoc
    : Data.IntSet.Internal.IntSet ->
      Data.IntSet.Internal.IntSet -> Data.IntSet.Internal.IntSet -> bool :=
   fun t1 t2 t3 =>
     Data.IntSet.Internal.union t1 (Data.IntSet.Internal.union t2 t3) GHC.Base.==
     Data.IntSet.Internal.union (Data.IntSet.Internal.union t1 t2) t3.
 
-Definition prop_UnionComm
+#[global] Definition prop_UnionComm
    : Data.IntSet.Internal.IntSet -> Data.IntSet.Internal.IntSet -> bool :=
   fun t1 t2 =>
     (Data.IntSet.Internal.union t1 t2 GHC.Base.== Data.IntSet.Internal.union t2 t1).
 
-Definition prop_Diff
+#[global] Definition prop_Diff
    : list Coq.Numbers.BinNums.N -> list Coq.Numbers.BinNums.N -> Prop :=
   fun xs ys =>
     let 't := Data.IntSet.Internal.difference (Data.IntSet.Internal.fromList xs)
@@ -208,7 +209,7 @@ Definition prop_Diff
      Data.OldList.sort (_Data.OldList.\\_ (Data.OldList.nub xs) (Data.OldList.nub
                                                                  ys))).
 
-Definition prop_Int
+#[global] Definition prop_Int
    : list Coq.Numbers.BinNums.N -> list Coq.Numbers.BinNums.N -> Prop :=
   fun xs ys =>
     let 't := Data.IntSet.Internal.intersection (Data.IntSet.Internal.fromList xs)
@@ -217,7 +218,7 @@ Definition prop_Int
     (Data.IntSet.Internal.toAscList t Test.QuickCheck.Property.===
      Data.OldList.sort (Data.OldList.nub ((Data.OldList.intersect) (xs) (ys)))).
 
-Definition prop_disjoint
+#[global] Definition prop_disjoint
    : Data.IntSet.Internal.IntSet -> Data.IntSet.Internal.IntSet -> bool :=
   fun a b =>
     Data.IntSet.Internal.disjoint a b GHC.Base.==
@@ -225,17 +226,17 @@ Definition prop_disjoint
 
 (* Skipping definition `IntSetProperties.prop_Ordered' *)
 
-Definition prop_List : list Coq.Numbers.BinNums.N -> bool :=
+#[global] Definition prop_List : list Coq.Numbers.BinNums.N -> bool :=
   fun xs =>
     (Data.OldList.sort (Data.OldList.nub xs) GHC.Base.==
      Data.IntSet.Internal.toAscList (Data.IntSet.Internal.fromList xs)).
 
-Definition prop_DescList : list Coq.Numbers.BinNums.N -> bool :=
+#[global] Definition prop_DescList : list Coq.Numbers.BinNums.N -> bool :=
   fun xs =>
     (GHC.List.reverse (Data.OldList.sort (Data.OldList.nub xs)) GHC.Base.==
      Data.IntSet.Internal.toDescList (Data.IntSet.Internal.fromList xs)).
 
-Definition prop_AscDescList : list Coq.Numbers.BinNums.N -> bool :=
+#[global] Definition prop_AscDescList : list Coq.Numbers.BinNums.N -> bool :=
   fun xs =>
     let s := Data.IntSet.Internal.fromList xs in
     Data.IntSet.Internal.toAscList s GHC.Base.==
@@ -243,7 +244,7 @@ Definition prop_AscDescList : list Coq.Numbers.BinNums.N -> bool :=
 
 (* Skipping definition `IntSetProperties.prop_fromList' *)
 
-Definition powersOf2 : Data.IntSet.Internal.IntSet :=
+#[global] Definition powersOf2 : Data.IntSet.Internal.IntSet :=
   Data.IntSet.Internal.fromList (Coq.Lists.List.flat_map (fun i =>
                                                             cons (Coq.NArith.BinNat.N.pow #2 i) nil)
                                                          (GHC.Enum.enumFromTo #0 #63)).
@@ -265,7 +266,7 @@ Fixpoint prop_Prefix (arg_0__ : Data.IntSet.Internal.IntSet) : bool
      | _ => true
      end.
 
-Definition prop_LeftRight : Data.IntSet.Internal.IntSet -> bool :=
+#[global] Definition prop_LeftRight : Data.IntSet.Internal.IntSet -> bool :=
   fun arg_0__ =>
     match arg_0__ with
     | Data.IntSet.Internal.Bin _ msk left_ right_ =>
@@ -278,34 +279,34 @@ Definition prop_LeftRight : Data.IntSet.Internal.IntSet -> bool :=
     | _ => true
     end.
 
-Definition toSet
+#[global] Definition toSet
    : Data.IntSet.Internal.IntSet ->
      Data.Set.Internal.Set_ Coq.Numbers.BinNums.N :=
   Data.Set.Internal.fromList GHC.Base.∘ Data.IntSet.Internal.toList.
 
-Definition prop_isProperSubsetOf
+#[global] Definition prop_isProperSubsetOf
    : Data.IntSet.Internal.IntSet -> Data.IntSet.Internal.IntSet -> bool :=
   fun a b =>
     Data.IntSet.Internal.isProperSubsetOf a b GHC.Base.==
     Data.Set.Internal.isProperSubsetOf (toSet a) (toSet b).
 
-Definition prop_isProperSubsetOf2
+#[global] Definition prop_isProperSubsetOf2
    : Data.IntSet.Internal.IntSet -> Data.IntSet.Internal.IntSet -> bool :=
   fun a b =>
     let c := Data.IntSet.Internal.union a b in
     Data.IntSet.Internal.isProperSubsetOf a c GHC.Base.== (a GHC.Base./= c).
 
-Definition prop_isSubsetOf
+#[global] Definition prop_isSubsetOf
    : Data.IntSet.Internal.IntSet -> Data.IntSet.Internal.IntSet -> bool :=
   fun a b =>
     Data.IntSet.Internal.isSubsetOf a b GHC.Base.==
     Data.Set.Internal.isSubsetOf (toSet a) (toSet b).
 
-Definition prop_isSubsetOf2
+#[global] Definition prop_isSubsetOf2
    : Data.IntSet.Internal.IntSet -> Data.IntSet.Internal.IntSet -> bool :=
   fun a b => Data.IntSet.Internal.isSubsetOf a (Data.IntSet.Internal.union a b).
 
-Definition prop_size : Data.IntSet.Internal.IntSet -> Prop :=
+#[global] Definition prop_size : Data.IntSet.Internal.IntSet -> Prop :=
   fun s =>
     let sz := Data.IntSet.Internal.size s in
     (sz Test.QuickCheck.Property.===
@@ -321,7 +322,7 @@ Definition prop_size : Data.IntSet.Internal.IntSet -> Prop :=
 
 (* Skipping definition `IntSetProperties.prop_findMin' *)
 
-Definition prop_ord
+#[global] Definition prop_ord
    : Data.IntSet.Internal.IntSet -> Data.IntSet.Internal.IntSet -> bool :=
   fun s1 s2 =>
     GHC.Base.compare s1 s2 GHC.Base.==
@@ -330,33 +331,33 @@ Definition prop_ord
 
 (* Skipping definition `IntSetProperties.prop_readShow' *)
 
-Definition prop_foldR : Data.IntSet.Internal.IntSet -> bool :=
+#[global] Definition prop_foldR : Data.IntSet.Internal.IntSet -> bool :=
   fun s =>
     Data.IntSet.Internal.foldr cons nil s GHC.Base.== Data.IntSet.Internal.toList s.
 
-Definition prop_foldR' : Data.IntSet.Internal.IntSet -> bool :=
+#[global] Definition prop_foldR' : Data.IntSet.Internal.IntSet -> bool :=
   fun s =>
     Data.IntSet.Internal.foldr' cons nil s GHC.Base.==
     Data.IntSet.Internal.toList s.
 
-Definition prop_foldL : Data.IntSet.Internal.IntSet -> bool :=
+#[global] Definition prop_foldL : Data.IntSet.Internal.IntSet -> bool :=
   fun s =>
     Data.IntSet.Internal.foldl (GHC.Base.flip cons) nil s GHC.Base.==
     Data.Foldable.foldl (GHC.Base.flip cons) nil (Data.IntSet.Internal.toList s).
 
-Definition prop_foldL' : Data.IntSet.Internal.IntSet -> bool :=
+#[global] Definition prop_foldL' : Data.IntSet.Internal.IntSet -> bool :=
   fun s =>
     Data.IntSet.Internal.foldl' (GHC.Base.flip cons) nil s GHC.Base.==
     Data.Foldable.foldl' (GHC.Base.flip cons) nil (Data.IntSet.Internal.toList s).
 
-Definition prop_map : Data.IntSet.Internal.IntSet -> bool :=
+#[global] Definition prop_map : Data.IntSet.Internal.IntSet -> bool :=
   fun s => Data.IntSet.Internal.map GHC.Base.id s GHC.Base.== s.
 
 (* Skipping definition `IntSetProperties.prop_maxView' *)
 
 (* Skipping definition `IntSetProperties.prop_minView' *)
 
-Definition prop_split
+#[global] Definition prop_split
    : Data.IntSet.Internal.IntSet -> Coq.Numbers.BinNums.N -> Prop :=
   fun s i =>
     let 'pair s1 s2 := Data.IntSet.Internal.split i s in
@@ -369,7 +370,7 @@ Definition prop_split
        (Data.IntSet.Internal.delete i s Test.QuickCheck.Property.===
         Data.IntSet.Internal.union s1 s2)))).
 
-Definition prop_splitMember
+#[global] Definition prop_splitMember
    : Data.IntSet.Internal.IntSet -> Coq.Numbers.BinNums.N -> Prop :=
   fun s i =>
     let 'pair (pair s1 t) s2 := Data.IntSet.Internal.splitMember i s in
@@ -384,7 +385,7 @@ Definition prop_splitMember
         (Data.IntSet.Internal.delete i s Test.QuickCheck.Property.===
          Data.IntSet.Internal.union s1 s2))))).
 
-Definition prop_splitRoot : Data.IntSet.Internal.IntSet -> bool :=
+#[global] Definition prop_splitRoot : Data.IntSet.Internal.IntSet -> bool :=
   fun s =>
     let loop :=
       fun arg_0__ =>
@@ -402,7 +403,7 @@ Definition prop_splitRoot : Data.IntSet.Internal.IntSet -> bool :=
     let ls := Data.IntSet.Internal.splitRoot s in
     andb (loop ls) (s GHC.Base.== Data.IntSet.Internal.unions ls).
 
-Definition prop_partition
+#[global] Definition prop_partition
    : Data.IntSet.Internal.IntSet -> Coq.Numbers.BinNums.N -> Prop :=
   fun s i =>
     let 'pair s1 s2 := Data.IntSet.Internal.partition GHC.Real.odd s in
@@ -414,7 +415,7 @@ Definition prop_partition
        Test.QuickCheck.Property..&&.(**)
        (s Test.QuickCheck.Property.=== Data.IntSet.Internal.union s1 s2)))).
 
-Definition prop_filter
+#[global] Definition prop_filter
    : Data.IntSet.Internal.IntSet -> Coq.Numbers.BinNums.N -> Prop :=
   fun s i =>
     let evens := Data.IntSet.Internal.filter GHC.Real.even s in
