examples/ghc/lib/Maybes.v
@@ -14,6 +14,7 @@ Require Coq.Program.Wf.
 
 Require Control.Monad.Trans.Maybe.
 Require Coq.Init.Datatypes.
+Require Data.Either.
 Require Data.Maybe.
 Require GHC.Base.
 Require GHC.Err.
@@ -32,7 +33,7 @@ Arguments Failed {_} {_} _.
 
 (* Converted value declarations: *)
 
-Local Definition Functor__MaybeErr_fmap {inst_err}
+#[local] Definition Functor__MaybeErr_fmap {inst_err}
    : forall {a} {b}, (a -> b) -> MaybeErr inst_err a -> MaybeErr inst_err b :=
   fun {a} {b} =>
     fun f x =>
@@ -41,11 +42,17 @@ Local Definition Functor__MaybeErr_fmap {inst_err}
       | Failed e => Failed e
       end.
 
-Local Definition Functor__MaybeErr_op_zlzd__ {inst_err : Type}
+#[local] Definition Functor__MaybeErr_op_zlzd__ {inst_err : Type}
    : forall {a : Type},
      forall {b : Type}, a -> MaybeErr inst_err b -> MaybeErr inst_err a :=
-  fun {a : Type} {b : Type} => Functor__MaybeErr_fmap GHC.Base.∘ GHC.Base.const.
+  fun {a : Type} {b : Type} =>
+    fun arg_0__ arg_1__ =>
+      match arg_0__, arg_1__ with
+      | z, Succeeded a1 => Succeeded ((fun b1 => z) a1)
+      | z, Failed a1 => Failed ((fun b1 => b1) a1)
+      end.
 
+#[global]
 Program Instance Functor__MaybeErr {err : Type}
    : GHC.Base.Functor (MaybeErr err) :=
   fun _ k__ =>
@@ -53,7 +60,7 @@ Program Instance Functor__MaybeErr {err : Type}
            GHC.Base.op_zlzd____ := fun {a : Type} {b : Type} =>
              Functor__MaybeErr_op_zlzd__ |}.
 
-Local Definition Applicative__MaybeErr_op_zlztzg__ {inst_err}
+#[local] Definition Applicative__MaybeErr_op_zlztzg__ {inst_err}
    : forall {a} {b},
      MaybeErr inst_err (a -> b) -> MaybeErr inst_err a -> MaybeErr inst_err b :=
   fun {a} {b} =>
@@ -67,7 +74,7 @@ Local Definition Applicative__MaybeErr_op_zlztzg__ {inst_err}
       | Failed e => Failed e
       end.
 
-Local Definition Applicative__MaybeErr_liftA2 {inst_err : Type}
+#[local] Definition Applicative__MaybeErr_liftA2 {inst_err : Type}
    : forall {a : Type},
      forall {b : Type},
      forall {c : Type},
@@ -76,17 +83,18 @@ Local Definition Applicative__MaybeErr_liftA2 {inst_err : Type}
   fun {a : Type} {b : Type} {c : Type} =>
     fun f x => Applicative__MaybeErr_op_zlztzg__ (GHC.Base.fmap f x).
 
-Local Definition Applicative__MaybeErr_op_ztzg__ {inst_err : Type}
+#[local] Definition Applicative__MaybeErr_op_ztzg__ {inst_err : Type}
    : forall {a : Type},
      forall {b : Type},
      MaybeErr inst_err a -> MaybeErr inst_err b -> MaybeErr inst_err b :=
   fun {a : Type} {b : Type} =>
     fun a1 a2 => Applicative__MaybeErr_op_zlztzg__ (GHC.Base.id GHC.Base.<$ a1) a2.
 
-Local Definition Applicative__MaybeErr_pure {inst_err : Type}
+#[local] Definition Applicative__MaybeErr_pure {inst_err : Type}
    : forall {a : Type}, a -> MaybeErr inst_err a :=
   fun {a : Type} => Succeeded.
 
+#[global]
 Program Instance Applicative__MaybeErr {err : Type}
    : GHC.Base.Applicative (MaybeErr err) :=
   fun _ k__ =>
@@ -98,7 +106,7 @@ Program Instance Applicative__MaybeErr {err : Type}
              Applicative__MaybeErr_op_ztzg__ ;
            GHC.Base.pure__ := fun {a : Type} => Applicative__MaybeErr_pure |}.
 
-Local Definition Monad__MaybeErr_op_zgzgze__ {inst_err : Type}
+#[local] Definition Monad__MaybeErr_op_zgzgze__ {inst_err : Type}
    : forall {a : Type},
      forall {b : Type},
      MaybeErr inst_err a -> (a -> MaybeErr inst_err b) -> MaybeErr inst_err b :=
@@ -109,17 +117,18 @@ Local Definition Monad__MaybeErr_op_zgzgze__ {inst_err : Type}
       | Failed e, _ => Failed e
       end.
 
-Local Definition Monad__MaybeErr_op_zgzg__ {inst_err : Type}
+#[local] Definition Monad__MaybeErr_op_zgzg__ {inst_err : Type}
    : forall {a : Type},
      forall {b : Type},
      MaybeErr inst_err a -> MaybeErr inst_err b -> MaybeErr inst_err b :=
   fun {a : Type} {b : Type} =>
     fun m k => Monad__MaybeErr_op_zgzgze__ m (fun arg_0__ => k).
 
-Local Definition Monad__MaybeErr_return_ {inst_err : Type}
+#[local] Definition Monad__MaybeErr_return_ {inst_err : Type}
    : forall {a : Type}, a -> MaybeErr inst_err a :=
   fun {a : Type} => GHC.Base.pure.
 
+#[global]
 Program Instance Monad__MaybeErr {err : Type} : GHC.Base.Monad (MaybeErr err) :=
   fun _ k__ =>
     k__ {| GHC.Base.op_zgzg____ := fun {a : Type} {b : Type} =>
@@ -132,7 +141,7 @@ Program Instance Monad__MaybeErr {err : Type} : GHC.Base.Monad (MaybeErr err) :=
 
 (* Skipping definition `Maybes.firstJusts' *)
 
-Definition expectJust {a} `{HsToCoq.Err.Default a}
+#[global] Definition expectJust {a} `{HsToCoq.Err.Default a}
    : GHC.Base.String -> option a -> a :=
   fun arg_0__ arg_1__ =>
     match arg_0__, arg_1__ with
@@ -141,7 +150,8 @@ Definition expectJust {a} `{HsToCoq.Err.Default a}
         GHC.Err.error (Coq.Init.Datatypes.app (GHC.Base.hs_string__ "expectJust ") err)
     end.
 
-Definition whenIsJust {m : Type -> Type} {a : Type} `{GHC.Base.Monad m}
+#[global] Definition whenIsJust {m : Type -> Type} {a : Type} `{GHC.Base.Monad
+  m}
    : option a -> (a -> m unit) -> m unit :=
   fun arg_0__ arg_1__ =>
     match arg_0__, arg_1__ with
@@ -149,28 +159,40 @@ Definition whenIsJust {m : Type -> Type} {a : Type} `{GHC.Base.Monad m}
     | None, _ => GHC.Base.return_ tt
     end.
 
-Definition orElse {a : Type} : option a -> a -> a :=
+#[global] Definition orElse {a : Type} : option a -> a -> a :=
   GHC.Base.flip Data.Maybe.fromMaybe.
 
-Definition liftMaybeT {m : Type -> Type} {a : Type} `{GHC.Base.Monad m}
+#[global] Definition rightToMaybe {a : Type} {b : Type}
+   : Data.Either.Either a b -> option b :=
+  fun arg_0__ =>
+    match arg_0__ with
+    | Data.Either.Left _ => None
+    | Data.Either.Right x => Some x
+    end.
+
+#[global] Definition liftMaybeT {m : Type -> Type} {a : Type} `{GHC.Base.Monad
+  m}
    : m a -> Control.Monad.Trans.Maybe.MaybeT m a :=
   fun act => Control.Monad.Trans.Maybe.Mk_MaybeT (GHC.Base.liftM Some act).
 
 (* Skipping definition `Maybes.tryMaybeT' *)
 
-Definition isSuccess {err : Type} {val : Type} : MaybeErr err val -> bool :=
+#[global] Definition isSuccess {err : Type} {val : Type}
+   : MaybeErr err val -> bool :=
   fun arg_0__ => match arg_0__ with | Succeeded _ => true | Failed _ => false end.
 
-Definition failME {err : Type} {val : Type} : err -> MaybeErr err val :=
+#[global] Definition failME {err : Type} {val : Type}
+   : err -> MaybeErr err val :=
   fun e => Failed e.
 
 (* External variables:
      None Some Type bool false option true tt unit Control.Monad.Trans.Maybe.MaybeT
-     Control.Monad.Trans.Maybe.Mk_MaybeT Coq.Init.Datatypes.app Data.Maybe.fromMaybe
-     GHC.Base.Applicative GHC.Base.Functor GHC.Base.Monad GHC.Base.String
-     GHC.Base.const GHC.Base.flip GHC.Base.fmap GHC.Base.fmap__ GHC.Base.id
-     GHC.Base.liftA2__ GHC.Base.liftM GHC.Base.op_z2218U__ GHC.Base.op_zgzg____
-     GHC.Base.op_zgzgze____ GHC.Base.op_zlzd__ GHC.Base.op_zlzd____
-     GHC.Base.op_zlztzg____ GHC.Base.op_ztzg____ GHC.Base.pure GHC.Base.pure__
-     GHC.Base.return_ GHC.Base.return___ GHC.Err.error HsToCoq.Err.Default
+     Control.Monad.Trans.Maybe.Mk_MaybeT Coq.Init.Datatypes.app Data.Either.Either
+     Data.Either.Left Data.Either.Right Data.Maybe.fromMaybe GHC.Base.Applicative
+     GHC.Base.Functor GHC.Base.Monad GHC.Base.String GHC.Base.flip GHC.Base.fmap
+     GHC.Base.fmap__ GHC.Base.id GHC.Base.liftA2__ GHC.Base.liftM
+     GHC.Base.op_zgzg____ GHC.Base.op_zgzgze____ GHC.Base.op_zlzd__
+     GHC.Base.op_zlzd____ GHC.Base.op_zlztzg____ GHC.Base.op_ztzg____ GHC.Base.pure
+     GHC.Base.pure__ GHC.Base.return_ GHC.Base.return___ GHC.Err.error
+     HsToCoq.Err.Default
 *)
