examples/ghc/lib/Util.v
@@ -16,28 +16,33 @@ Require HsToCoq.Nat.
 
 (* Converted imports: *)
 
+Require Control.Monad.IO.Class.
 Require Coq.Init.Datatypes.
 Require Coq.Lists.List.
 Require Data.Bits.
 Require Data.Either.
 Require Data.Foldable.
+Require Data.Functor.
 Require Data.OldList.
+Require Data.Set.Internal.
 Require GHC.Base.
 Require GHC.Char.
+Require GHC.Enum.
 Require GHC.Err.
 Require GHC.List.
 Require GHC.Num.
 Require GHC.Prim.
 Require HsToCoq.DeferredFix.
 Require HsToCoq.Err.
-Require Panic.
+Require PlainPanic.
 Import Data.Bits.Notations.
+Import Data.Functor.Notations.
 Import GHC.Base.Notations.
 Import GHC.Num.Notations.
 
 (* Converted type declarations: *)
 
-Definition Suffix :=
+#[global] Definition Suffix :=
   GHC.Base.String%type.
 
 Inductive OverridingBool : Type :=
@@ -45,7 +50,7 @@ Inductive OverridingBool : Type :=
   | Always : OverridingBool
   | Never : OverridingBool.
 
-Definition HasDebugCallStack :=
+#[global] Definition HasDebugCallStack :=
   unit.
 
 Inductive Direction : Type := | Forwards : Direction | Backwards : Direction.
@@ -66,76 +71,83 @@ Instance Util_HasDebugCallStack : HasDebugCallStack := tt.
 (* Skipping all instances of class `GHC.Show.Show', including
    `Util.Show__OverridingBool' *)
 
-Definition ghciSupported : bool :=
+#[global] Definition ghciSupported : bool :=
   false.
 
 Axiom debugIsOn : bool.
 
-Definition ncgDebugIsOn : bool :=
+#[global] Definition ghciTablesNextToCode : bool :=
   false.
 
-Definition ghciTablesNextToCode : bool :=
-  false.
-
-Definition isWindowsHost : bool :=
+#[global] Definition isWindowsHost : bool :=
   false.
 
 (* Skipping definition `Util.isDarwinHost' *)
 
+#[global] Definition applyWhen {a : Type} : bool -> (a -> a) -> a -> a :=
+  fun arg_0__ arg_1__ arg_2__ =>
+    match arg_0__, arg_1__, arg_2__ with
+    | true, f, x => f x
+    | _, _, x => x
+    end.
+
 (* Skipping definition `Util.nTimes' *)
 
-Definition fstOf3 {a : Type} {b : Type} {c : Type} : (a * b * c)%type -> a :=
+#[global] Definition fstOf3 {a : Type} {b : Type} {c : Type}
+   : (a * b * c)%type -> a :=
   fun '(pair (pair a _) _) => a.
 
-Definition sndOf3 {a : Type} {b : Type} {c : Type} : (a * b * c)%type -> b :=
+#[global] Definition sndOf3 {a : Type} {b : Type} {c : Type}
+   : (a * b * c)%type -> b :=
   fun '(pair (pair _ b) _) => b.
 
-Definition thdOf3 {a : Type} {b : Type} {c : Type} : (a * b * c)%type -> c :=
+#[global] Definition thdOf3 {a : Type} {b : Type} {c : Type}
+   : (a * b * c)%type -> c :=
   fun '(pair (pair _ _) c) => c.
 
-Definition fst3 {a : Type} {d : Type} {b : Type} {c : Type}
+#[global] Definition fst3 {a : Type} {d : Type} {b : Type} {c : Type}
    : (a -> d) -> (a * b * c)%type -> (d * b * c)%type :=
   fun arg_0__ arg_1__ =>
     match arg_0__, arg_1__ with
     | f, pair (pair a b) c => pair (pair (f a) b) c
     end.
 
-Definition snd3 {b : Type} {d : Type} {a : Type} {c : Type}
+#[global] Definition snd3 {b : Type} {d : Type} {a : Type} {c : Type}
    : (b -> d) -> (a * b * c)%type -> (a * d * c)%type :=
   fun arg_0__ arg_1__ =>
     match arg_0__, arg_1__ with
     | f, pair (pair a b) c => pair (pair a (f b)) c
     end.
 
-Definition third3 {c : Type} {d : Type} {a : Type} {b : Type}
+#[global] Definition third3 {c : Type} {d : Type} {a : Type} {b : Type}
    : (c -> d) -> (a * b * c)%type -> (a * b * d)%type :=
   fun arg_0__ arg_1__ =>
     match arg_0__, arg_1__ with
     | f, pair (pair a b) c => pair (pair a b) (f c)
     end.
 
-Definition uncurry3 {a : Type} {b : Type} {c : Type} {d : Type}
+#[global] Definition uncurry3 {a : Type} {b : Type} {c : Type} {d : Type}
    : (a -> b -> c -> d) -> (a * b * c)%type -> d :=
   fun arg_0__ arg_1__ =>
     match arg_0__, arg_1__ with
     | f, pair (pair a b) c => f a b c
     end.
 
-Definition liftFst {a : Type} {b : Type} {c : Type}
+#[global] Definition liftFst {a : Type} {b : Type} {c : Type}
    : (a -> b) -> (a * c)%type -> (b * c)%type :=
   fun arg_0__ arg_1__ =>
     match arg_0__, arg_1__ with
     | f, pair a c => pair (f a) c
     end.
 
-Definition liftSnd {a : Type} {b : Type} {c : Type}
+#[global] Definition liftSnd {a : Type} {b : Type} {c : Type}
    : (a -> b) -> (c * a)%type -> (c * b)%type :=
   fun arg_0__ arg_1__ =>
     match arg_0__, arg_1__ with
     | f, pair c a => pair c (f a)
     end.
 
-Definition firstM {m : Type -> Type} {a : Type} {c : Type} {b : Type}
+#[global] Definition firstM {m : Type -> Type} {a : Type} {c : Type} {b : Type}
   `{GHC.Base.Monad m}
    : (a -> m c) -> (a * b)%type -> m (c * b)%type :=
   fun arg_0__ arg_1__ =>
@@ -143,12 +155,20 @@ Definition firstM {m : Type -> Type} {a : Type} {c : Type} {b : Type}
     | f, pair x y => GHC.Base.liftM (fun x' => pair x' y) (f x)
     end.
 
-Definition first3M {m : Type -> Type} {a : Type} {d : Type} {b : Type} {c
-   : Type} `{GHC.Base.Monad m}
+#[global] Definition first3M {m : Type -> Type} {a : Type} {d : Type} {b : Type}
+  {c : Type} `{GHC.Base.Monad m}
    : (a -> m d) -> (a * b * c)%type -> m (d * b * c)%type :=
   fun arg_0__ arg_1__ =>
     match arg_0__, arg_1__ with
     | f, pair (pair x y) z => GHC.Base.liftM (fun x' => pair (pair x' y) z) (f x)
+    end.
+
+#[global] Definition secondM {m : Type -> Type} {b : Type} {c : Type} {a : Type}
+  `{GHC.Base.Monad m}
+   : (b -> m c) -> (a * b)%type -> m (a * c)%type :=
+  fun arg_0__ arg_1__ =>
+    match arg_0__, arg_1__ with
+    | f, pair x y => (fun arg_2__ => pair x arg_2__) Data.Functor.<$> f y
     end.
 
 Fixpoint filterOut {a : Type} (arg_0__ : a -> bool) (arg_1__ : list a) : list a
@@ -169,37 +189,26 @@ Fixpoint partitionWith {a : Type} {b : Type} {c : Type} (arg_0__
          end
      end.
 
-Fixpoint splitEithers {a : Type} {b : Type} (arg_0__
-                        : list (Data.Either.Either a b)) : (list a * list b)%type
-  := match arg_0__ with
-     | nil => pair nil nil
-     | cons e es =>
-         let 'pair xs ys := splitEithers es in
-         match e with
-         | Data.Either.Left x => pair (cons x xs) ys
-         | Data.Either.Right y => pair xs (cons y ys)
-         end
-     end.
-
-Definition chkAppend {a : Type} : list a -> list a -> list a :=
+#[global] Definition chkAppend {a : Type} : list a -> list a -> list a :=
   fun xs ys =>
     if Data.Foldable.null ys : bool then xs else
     Coq.Init.Datatypes.app xs ys.
 
-Definition zipEqual {a : Type} {b : Type}
+#[global] Definition zipEqual {a : Type} {b : Type}
    : GHC.Base.String -> list a -> list b -> list (a * b)%type :=
   fun arg_0__ => GHC.List.zip.
 
-Definition zipWithEqual {a : Type} {b : Type} {c : Type}
+#[global] Definition zipWithEqual {a : Type} {b : Type} {c : Type}
    : GHC.Base.String -> (a -> b -> c) -> list a -> list b -> list c :=
   fun arg_0__ => GHC.List.zipWith.
 
-Definition zipWith3Equal {a : Type} {b : Type} {c : Type} {d : Type}
+#[global] Definition zipWith3Equal {a : Type} {b : Type} {c : Type} {d : Type}
    : GHC.Base.String ->
      (a -> b -> c -> d) -> list a -> list b -> list c -> list d :=
   fun arg_0__ => GHC.List.zipWith3.
 
-Definition zipWith4Equal {a : Type} {b : Type} {c : Type} {d : Type} {e : Type}
+#[global] Definition zipWith4Equal {a : Type} {b : Type} {c : Type} {d : Type}
+  {e : Type}
    : GHC.Base.String ->
      (a -> b -> c -> d -> e) -> list a -> list b -> list c -> list d -> list e :=
   fun arg_0__ => Data.OldList.zipWith4.
@@ -246,7 +255,7 @@ Fixpoint filterByLists {a : Type} (arg_0__ : list bool) (arg_1__ arg_2__
      | _, _, _ => nil
      end.
 
-Definition partitionByList {a : Type}
+#[global] Definition partitionByList {a : Type}
    : list bool -> list a -> (list a * list a)%type :=
   let fix go arg_0__ arg_1__ arg_2__ arg_3__
     := match arg_0__, arg_1__, arg_2__, arg_3__ with
@@ -269,13 +278,13 @@ Fixpoint stretchZipWith {a : Type} {b : Type} {c : Type} (arg_0__ : a -> bool)
          end
      end.
 
-Definition mapFst {a : Type} {c : Type} {b : Type}
+#[global] Definition mapFst {a : Type} {c : Type} {b : Type}
    : (a -> c) -> list (a * b)%type -> list (c * b)%type :=
   fun f xys =>
     let cont_0__ arg_1__ := let 'pair x y := arg_1__ in cons (pair (f x) y) nil in
     Coq.Lists.List.flat_map cont_0__ xys.
 
-Definition mapSnd {b : Type} {c : Type} {a : Type}
+#[global] Definition mapSnd {b : Type} {c : Type} {a : Type}
    : (b -> c) -> list (a * b)%type -> list (a * c)%type :=
   fun f xys =>
     let cont_0__ arg_1__ := let 'pair x y := arg_1__ in cons (pair x (f y)) nil in
@@ -312,12 +321,18 @@ Fixpoint zipWithAndUnzip {a : Type} {b : Type} {c : Type} {d : Type} (arg_0__
      | _, _, _ => pair nil nil
      end.
 
+Fixpoint zipAndUnzip {a : Type} {b : Type} (arg_0__ : list a) (arg_1__ : list b)
+  : (list a * list b)%type
+  := match arg_0__, arg_1__ with
+     | cons a as_, cons b bs =>
+         let 'pair rs1 rs2 := zipAndUnzip as_ bs in
+         pair (cons a rs1) (cons b rs2)
+     | _, _ => pair nil nil
+     end.
+
 (* Skipping definition `Util.mapAccumL2' *)
 
-Definition nOfThem {a : Type} : nat -> a -> list a :=
-  fun n thing => Coq.Lists.List.repeat thing n.
-
-Definition atLength {a : Type} {b : Type}
+#[global] Definition atLength {a : Type} {b : Type}
    : (list a -> b) -> b -> list a -> nat -> b :=
   fun atLenPred atEnd ls0 n0 =>
     let fix go arg_0__ arg_1__
@@ -332,36 +347,36 @@ Definition atLength {a : Type} {b : Type}
     if n0 GHC.Base.< #0 : bool then atLenPred ls0 else
     go n0 ls0.
 
-Definition notNull {a : Type} : list a -> bool :=
+#[global] Definition notNull {a : Type} : list a -> bool :=
   fun arg_0__ => match arg_0__ with | nil => false | _ => true end.
 
-Definition lengthExceeds {a : Type} : list a -> nat -> bool :=
+#[global] Definition lengthExceeds {a : Type} : list a -> nat -> bool :=
   fun lst n =>
     if n GHC.Base.< #0 : bool then true else
     atLength notNull false lst n.
 
-Definition lengthAtLeast {a : Type} : list a -> nat -> bool :=
+#[global] Definition lengthAtLeast {a : Type} : list a -> nat -> bool :=
   atLength (GHC.Base.const true) false.
 
-Definition lengthIs {a : Type} : list a -> nat -> bool :=
+#[global] Definition lengthIs {a : Type} : list a -> nat -> bool :=
   fun lst n =>
     if n GHC.Base.< #0 : bool then false else
     atLength Data.Foldable.null false lst n.
 
-Definition lengthIsNot {a : Type} : list a -> nat -> bool :=
+#[global] Definition lengthIsNot {a : Type} : list a -> nat -> bool :=
   fun lst n =>
     if n GHC.Base.< #0 : bool then true else
     atLength notNull true lst n.
 
-Definition lengthAtMost {a : Type} : list a -> nat -> bool :=
+#[global] Definition lengthAtMost {a : Type} : list a -> nat -> bool :=
   fun lst n =>
     if n GHC.Base.< #0 : bool then false else
     atLength Data.Foldable.null true lst n.
 
-Definition lengthLessThan {a : Type} : list a -> nat -> bool :=
+#[global] Definition lengthLessThan {a : Type} : list a -> nat -> bool :=
   atLength (GHC.Base.const false) true.
 
-Definition listLengthCmp {a : Type} : list a -> nat -> comparison :=
+#[global] Definition listLengthCmp {a : Type} : list a -> nat -> comparison :=
   let atLen := fun arg_0__ => match arg_0__ with | nil => Eq | _ => Gt end in
   let atEnd := Lt in atLength atLen atEnd.
 
@@ -373,14 +388,6 @@ Fixpoint equalLength {a : Type} {b : Type} (arg_0__ : list a) (arg_1__ : list b)
      | _, _ => false
      end.
 
-Fixpoint neLength {a : Type} {b : Type} (arg_0__ : list a) (arg_1__ : list b)
-  : bool
-  := match arg_0__, arg_1__ with
-     | nil, nil => false
-     | cons _ xs, cons _ ys => neLength xs ys
-     | _, _ => true
-     end.
-
 Fixpoint compareLength {a : Type} {b : Type} (arg_0__ : list a) (arg_1__
                          : list b) : comparison
   := match arg_0__, arg_1__ with
@@ -390,7 +397,8 @@ Fixpoint compareLength {a : Type} {b : Type} (arg_0__ : list a) (arg_1__
      | _, nil => Gt
      end.
 
-Definition leLength {a : Type} {b : Type} : list a -> list b -> bool :=
+#[global] Definition leLength {a : Type} {b : Type}
+   : list a -> list b -> bool :=
   fun xs ys =>
     match compareLength xs ys with
     | Lt => true
@@ -398,7 +406,8 @@ Definition leLength {a : Type} {b : Type} : list a -> list b -> bool :=
     | Gt => false
     end.
 
-Definition ltLength {a : Type} {b : Type} : list a -> list b -> bool :=
+#[global] Definition ltLength {a : Type} {b : Type}
+   : list a -> list b -> bool :=
   fun xs ys =>
     match compareLength xs ys with
     | Lt => true
@@ -406,24 +415,24 @@ Definition ltLength {a : Type} {b : Type} : list a -> list b -> bool :=
     | Gt => false
     end.
 
-Definition singleton {a : Type} : a -> list a :=
+#[global] Definition singleton {a : Type} : a -> list a :=
   fun x => cons x nil.
 
-Definition isSingleton {a : Type} : list a -> bool :=
+#[global] Definition isSingleton {a : Type} : list a -> bool :=
   fun arg_0__ => match arg_0__ with | cons _ nil => true | _ => false end.
 
-Definition only {a} `{HsToCoq.Err.Default a} : list a -> a :=
+#[global] Definition only {a} `{HsToCoq.Err.Default a} : list a -> a :=
   fun arg_0__ =>
     match arg_0__ with
     | cons a _ => a
-    | _ => Panic.panic (GHC.Base.hs_string__ "Util: only")
+    | _ => PlainPanic.panic (GHC.Base.hs_string__ "Util: only")
     end.
 
-Definition isIn {a : Type} `{GHC.Base.Eq_ a}
+#[global] Definition isIn {a : Type} `{GHC.Base.Eq_ a}
    : GHC.Base.String -> a -> list a -> bool :=
   fun _msg x ys => Data.Foldable.elem x ys.
 
-Definition isn'tIn {a : Type} `{GHC.Base.Eq_ a}
+#[global] Definition isn'tIn {a : Type} `{GHC.Base.Eq_ a}
    : GHC.Base.String -> a -> list a -> bool :=
   fun _msg x ys => Data.Foldable.notElem x ys.
 
@@ -431,16 +440,36 @@ Definition isn'tIn {a : Type} `{GHC.Base.Eq_ a}
 
 Fixpoint changeLast {a : Type} (arg_0__ : list a) (arg_1__ : a) : list a
   := match arg_0__, arg_1__ with
-     | nil, _ => Panic.panic (GHC.Base.hs_string__ "changeLast")
+     | nil, _ => PlainPanic.panic (GHC.Base.hs_string__ "changeLast")
      | cons _ nil, x => cons x nil
      | cons x xs, x' => cons x (changeLast xs x')
      end.
+
+#[global] Definition whenNonEmpty {m : Type -> Type} {a : Type}
+  `{GHC.Base.Applicative m}
+   : list a -> (GHC.Base.NonEmpty a -> m unit) -> m unit :=
+  fun arg_0__ arg_1__ =>
+    match arg_0__, arg_1__ with
+    | nil, _ => GHC.Base.pure tt
+    | cons x xs, f => f (GHC.Base.NEcons x xs)
+    end.
 
 (* Skipping definition `Util.minWith' *)
 
 (* Skipping definition `Util.nubSort' *)
 
-Definition transitiveClosure {a : Type}
+#[global] Definition ordNub {a : Type} `{GHC.Base.Ord a} : list a -> list a :=
+  fun xs =>
+    let fix go arg_0__ arg_1__
+      := match arg_0__, arg_1__ with
+         | _, nil => nil
+         | s, cons x xs =>
+             if Data.Set.Internal.member x s : bool then go s xs else
+             cons x (go (Data.Set.Internal.insert x s) xs)
+         end in
+    go Data.Set.Internal.empty xs.
+
+#[global] Definition transitiveClosure {a : Type}
    : (a -> list a) -> (a -> a -> bool) -> list a -> list a :=
   fun succ eq xs =>
     let fix is_in arg_0__ arg_1__
@@ -464,7 +493,7 @@ Fixpoint foldl2 {acc} {a} {b} `{HsToCoq.Err.Default acc} (arg_0__
   := match arg_0__, arg_1__, arg_2__, arg_3__ with
      | _, z, nil, nil => z
      | k, z, cons a as_, cons b bs => foldl2 k (k z a b) as_ bs
-     | _, _, _, _ => Panic.panic (GHC.Base.hs_string__ "Util: foldl2")
+     | _, _, _, _ => PlainPanic.panic (GHC.Base.hs_string__ "Util: foldl2")
      end.
 
 Fixpoint all2 {a : Type} {b : Type} (arg_0__ : a -> b -> bool) (arg_1__
@@ -475,12 +504,22 @@ Fixpoint all2 {a : Type} {b : Type} (arg_0__ : a -> b -> bool) (arg_1__
      | _, _, _ => false
      end.
 
-Definition count {a : Type} : (a -> bool) -> list a -> nat :=
+#[global] Definition count {a : Type} : (a -> bool) -> list a -> nat :=
   fun p =>
     let fix go arg_0__ arg_1__
       := match arg_0__, arg_1__ with
          | n, nil => n
          | n, cons x xs => if p x : bool then go (n GHC.Num.+ #1) xs else go n xs
+         end in
+    go #0.
+
+#[global] Definition countWhile {a : Type} : (a -> bool) -> list a -> nat :=
+  fun p =>
+    let fix go arg_0__ arg_1__
+      := let j_2__ := match arg_0__, arg_1__ with | n, _ => n end in
+         match arg_0__, arg_1__ with
+         | n, cons x xs => if p x : bool then go (n GHC.Num.+ #1) xs else j_2__
+         | _, _ => j_2__
          end in
     go #0.
 
@@ -513,7 +552,7 @@ Fixpoint splitAtList {b : Type} {a : Type} (arg_0__ : list b) (arg_1__ : list a)
          pair (cons y ys') ys''
      end.
 
-Definition dropTail {a : Type} : nat -> list a -> list a :=
+#[global] Definition dropTail {a : Type} : nat -> list a -> list a :=
   fun n xs =>
     let fix go arg_0__ arg_1__
       := match arg_0__, arg_1__ with
@@ -522,14 +561,15 @@ Definition dropTail {a : Type} : nat -> list a -> list a :=
          end in
     go (Coq.Lists.List.skipn n xs) xs.
 
-Definition dropWhileEndLE {a : Type} : (a -> bool) -> list a -> list a :=
+#[global] Definition dropWhileEndLE {a : Type}
+   : (a -> bool) -> list a -> list a :=
   fun p =>
     Data.Foldable.foldr (fun x r =>
                            if andb (Data.Foldable.null r) (p x) : bool
                            then nil
                            else cons x r) nil.
 
-Definition spanEnd {a : Type}
+#[global] Definition spanEnd {a : Type}
    : (a -> bool) -> list a -> (list a * list a)%type :=
   fun p l =>
     let fix go arg_0__ arg_1__ arg_2__ arg_3__
@@ -541,21 +581,39 @@ Definition spanEnd {a : Type}
          end in
     go l nil nil l.
 
-Definition snocView {a : Type} : list a -> option (list a * a)%type :=
+#[global] Definition last2 {a : Type} : list a -> (a * a)%type :=
+  let partialError :=
+    PlainPanic.panic (GHC.Base.hs_string__ "last2 - list length less than two") in
+  Data.Foldable.foldl' (fun arg_1__ arg_2__ =>
+                          match arg_1__, arg_2__ with
+                          | pair _ x2, x => pair x2 x
+                          end) (pair partialError partialError).
+
+#[global] Definition lastMaybe {a : Type} : list a -> option a :=
+  fun arg_0__ =>
+    match arg_0__ with
+    | nil => None
+    | xs => Some (GHC.List.last xs)
+    end.
+
+#[global] Definition snocView {a : Type} : list a -> option (list a * a)%type :=
   fun arg_0__ =>
     match arg_0__ with
     | nil => None
     | xs =>
-        let fix go arg_1__ arg_2__
-          := match arg_1__, arg_2__ with
-             | acc, cons x nil => Some (pair (GHC.List.reverse acc) x)
-             | acc, cons x xs => go (cons x acc) xs
-             | _, nil => Panic.panic (GHC.Base.hs_string__ "Util: snocView")
-             end in
-        go nil xs
+        let go {a} : list a -> (list a * a)%type :=
+          fix go (arg_1__ : list a) : (list a * a)%type
+            := match arg_1__ with
+               | cons x nil => pair nil x
+               | cons x xs => let 'pair xs' x' := go xs in pair (cons x xs') x'
+               | nil => GHC.Err.error (GHC.Base.hs_string__ "impossible")
+               end in
+        let 'pair xs x := go xs in
+        Some (pair xs x)
     end.
 
-Definition split : GHC.Char.Char -> GHC.Base.String -> list GHC.Base.String :=
+#[global] Definition split
+   : GHC.Char.Char -> GHC.Base.String -> list GHC.Base.String :=
   HsToCoq.DeferredFix.deferredFix2 (fun split
                                     (c : GHC.Char.Char)
                                     (s : GHC.Base.String) =>
@@ -566,13 +624,13 @@ Definition split : GHC.Char.Char -> GHC.Base.String -> list GHC.Base.String :=
                                       | cons _ rest => cons chunk (split c rest)
                                       end).
 
-Definition capitalise : GHC.Base.String -> GHC.Base.String :=
+#[global] Definition capitalise : GHC.Base.String -> GHC.Base.String :=
   fun arg_0__ => match arg_0__ with | nil => nil | cons c cs => cons c cs end.
 
-Definition isEqual : comparison -> bool :=
+#[global] Definition isEqual : comparison -> bool :=
   fun arg_0__ => match arg_0__ with | Gt => false | Eq => true | Lt => false end.
 
-Definition thenCmp : comparison -> comparison -> comparison :=
+#[global] Definition thenCmp : comparison -> comparison -> comparison :=
   fun arg_0__ arg_1__ =>
     match arg_0__, arg_1__ with
     | Eq, ordering => ordering
@@ -587,7 +645,7 @@ Fixpoint eqListBy {a : Type} (arg_0__ : a -> a -> bool) (arg_1__ arg_2__
      | _, _, _ => false
      end.
 
-Definition eqMaybeBy {a : Type}
+#[global] Definition eqMaybeBy {a : Type}
    : (a -> a -> bool) -> option a -> option a -> bool :=
   fun arg_0__ arg_1__ arg_2__ =>
     match arg_0__, arg_1__, arg_2__ with
@@ -611,7 +669,7 @@ Fixpoint cmpList {a : Type} (arg_0__ : a -> a -> comparison) (arg_1__ arg_2__
 
 (* Skipping definition `Util.removeSpaces' *)
 
-Definition op_zlzazazg__ {f : Type -> Type} `{GHC.Base.Applicative f}
+#[global] Definition op_zlzazazg__ {f : Type -> Type} `{GHC.Base.Applicative f}
    : f bool -> f bool -> f bool :=
   GHC.Base.liftA2 andb.
 
@@ -619,7 +677,7 @@ Notation "'_<&&>_'" := (op_zlzazazg__).
 
 Infix "<&&>" := (_<&&>_) (at level 99).
 
-Definition op_zlzbzbzg__ {f : Type -> Type} `{GHC.Base.Applicative f}
+#[global] Definition op_zlzbzbzg__ {f : Type -> Type} `{GHC.Base.Applicative f}
    : f bool -> f bool -> f bool :=
   GHC.Base.liftA2 orb.
 
@@ -635,7 +693,8 @@ Infix "<||>" := (_<||>_) (at level 99).
 
 (* Skipping definition `Util.restrictedDamerauLevenshteinDistanceWorker' *)
 
-Definition sizedComplement {bv} `{Data.Bits.Bits bv} : bv -> bv -> bv :=
+#[global] Definition sizedComplement {bv} `{Data.Bits.Bits bv}
+   : bv -> bv -> bv :=
   fun vector_mask vect => Data.Bits.xor vector_mask vect.
 
 (* Skipping definition `Util.matchVectors' *)
@@ -644,7 +703,7 @@ Definition sizedComplement {bv} `{Data.Bits.Bits bv} : bv -> bv -> bv :=
 
 (* Skipping definition `Util.fuzzyLookup' *)
 
-Definition unzipWith {a : Type} {b : Type} {c : Type}
+#[global] Definition unzipWith {a : Type} {b : Type} {c : Type}
    : (a -> b -> c) -> list (a * b)%type -> list c :=
   fun f pairs => GHC.Base.map (fun '(pair a b) => f a b) pairs.
 
@@ -674,17 +733,16 @@ Axiom looksLikePackageName : GHC.Base.String -> bool.
 
 (* Skipping definition `Util.toArgs' *)
 
-Definition exactLog2 : GHC.Num.Integer -> option GHC.Num.Integer :=
+#[global] Definition exactLog2 : GHC.Num.Integer -> option GHC.Num.Integer :=
   fun x =>
-    let pow2 :=
-      HsToCoq.DeferredFix.deferredFix1 (fun pow2 x =>
-                                          if x GHC.Base.== #1 : bool then #0 else
-                                          #1 GHC.Num.+ pow2 (Data.Bits.shiftR x #1)) in
-    if (orb (x GHC.Base.<= #0) (x GHC.Base.>= #2147483648)) : bool
-    then None
-    else if (x Data.Bits..&.(**) (GHC.Num.negate x)) GHC.Base./= x : bool
-         then None
-         else Some (pow2 x).
+    let x' := GHC.Real.fromIntegral x : GHC.Int.Int32 in
+    let c := Data.Bits.countTrailingZeros x' in
+    if x GHC.Base.<= #0 : bool then None else
+    if x GHC.Base.> GHC.Real.fromIntegral (GHC.Enum.maxBound : GHC.Int.Int32) : bool
+    then None else
+    if (x' Data.Bits..&.(**) (GHC.Num.negate x')) GHC.Base./= x' : bool
+    then None else
+    Some (GHC.Real.fromIntegral c).
 
 (* Skipping definition `Util.readRational__' *)
 
@@ -694,17 +752,26 @@ Definition exactLog2 : GHC.Num.Integer -> option GHC.Num.Integer :=
 
 (* Skipping definition `Util.readHexRational__' *)
 
-(* Skipping definition `Util.maybeRead' *)
-
-(* Skipping definition `Util.maybeReadFuzzy' *)
-
 (* Skipping definition `Util.doesDirNameExist' *)
 
 (* Skipping definition `Util.getModificationUTCTime' *)
 
 (* Skipping definition `Util.modificationTimeIfExists' *)
 
-(* Skipping definition `Util.hSetTranslit' *)
+#[global] Definition withAtomicRename {m : Type -> Type} {a : Type}
+  `{Control.Monad.IO.Class.MonadIO m}
+   : GHC.Base.String -> (GHC.Base.String -> m a) -> m a :=
+  fun targetFile f =>
+    let enableAtomicRename : bool := true in
+    if enableAtomicRename : bool
+    then let temp :=
+           targetFile System.FilePath.Posix.<.> GHC.Base.hs_string__ "tmp" in
+         f temp GHC.Base.>>=
+         (fun res =>
+            Control.Monad.IO.Class.liftIO (System.Directory.renameFile temp targetFile)
+            GHC.Base.>>
+            GHC.Base.return_ res) else
+    f targetFile.
 
 (* Skipping definition `Util.splitLongestPrefix' *)
 
@@ -728,7 +795,7 @@ Axiom makeRelativeTo : GHC.Base.String -> GHC.Base.String -> GHC.Base.String.
 
 (* Skipping definition `Util.mulHi' *)
 
-Definition overrideWith : bool -> OverridingBool -> bool :=
+#[global] Definition overrideWith : bool -> OverridingBool -> bool :=
   fun arg_0__ arg_1__ =>
     match arg_0__, arg_1__ with
     | b, Auto => b
@@ -745,17 +812,22 @@ End Notations.
 
 (* External variables:
      Eq Gt Lt None Some Type andb bool comparison cons false list nat nil op_zt__
-     option orb pair true unit Coq.Init.Datatypes.app Coq.Lists.List.flat_map
-     Coq.Lists.List.repeat Coq.Lists.List.skipn Data.Bits.Bits Data.Bits.op_zizazi__
-     Data.Bits.shiftR Data.Bits.xor Data.Either.Either Data.Either.Left
-     Data.Either.Right Data.Foldable.elem Data.Foldable.foldr Data.Foldable.notElem
-     Data.Foldable.null Data.OldList.zipWith4 GHC.Base.Applicative GHC.Base.Eq_
-     GHC.Base.Monad GHC.Base.String GHC.Base.const GHC.Base.liftA2 GHC.Base.liftM
-     GHC.Base.map GHC.Base.op_zeze__ GHC.Base.op_zgze__ GHC.Base.op_zl__
-     GHC.Base.op_zlze__ GHC.Base.op_zsze__ GHC.Char.Char GHC.Err.patternFailure
-     GHC.List.break GHC.List.reverse GHC.List.zip GHC.List.zipWith GHC.List.zipWith3
-     GHC.Num.Integer GHC.Num.fromInteger GHC.Num.negate GHC.Num.op_zm__
-     GHC.Num.op_zp__ GHC.Prim.seq HsToCoq.DeferredFix.deferredFix1
+     option orb pair true tt unit Control.Monad.IO.Class.MonadIO
+     Control.Monad.IO.Class.liftIO Coq.Init.Datatypes.app Coq.Lists.List.flat_map
+     Coq.Lists.List.skipn Data.Bits.Bits Data.Bits.countTrailingZeros
+     Data.Bits.op_zizazi__ Data.Bits.xor Data.Either.Either Data.Either.Left
+     Data.Either.Right Data.Foldable.elem Data.Foldable.foldl' Data.Foldable.foldr
+     Data.Foldable.notElem Data.Foldable.null Data.Functor.op_zlzdzg__
+     Data.OldList.zipWith4 Data.Set.Internal.empty Data.Set.Internal.insert
+     Data.Set.Internal.member GHC.Base.Applicative GHC.Base.Eq_ GHC.Base.Monad
+     GHC.Base.NEcons GHC.Base.NonEmpty GHC.Base.Ord GHC.Base.String GHC.Base.const
+     GHC.Base.liftA2 GHC.Base.liftM GHC.Base.map GHC.Base.op_zeze__ GHC.Base.op_zg__
+     GHC.Base.op_zgzg__ GHC.Base.op_zgzgze__ GHC.Base.op_zl__ GHC.Base.op_zlze__
+     GHC.Base.op_zsze__ GHC.Base.pure GHC.Base.return_ GHC.Char.Char
+     GHC.Enum.maxBound GHC.Err.error GHC.Err.patternFailure GHC.Int.Int32
+     GHC.List.break GHC.List.last GHC.List.reverse GHC.List.zip GHC.List.zipWith
+     GHC.List.zipWith3 GHC.Num.Integer GHC.Num.fromInteger GHC.Num.negate
+     GHC.Num.op_zm__ GHC.Num.op_zp__ GHC.Prim.seq GHC.Real.fromIntegral
      HsToCoq.DeferredFix.deferredFix2 HsToCoq.Err.Build_Default HsToCoq.Err.Default
-     Panic.panic
+     PlainPanic.panic System.Directory.renameFile System.FilePath.Posix.op_zlzizg__
 *)
